New class attempt

model/noc.dfy
@@ -3,7 +3,7 @@ module NoC {
 
   const BUFFER_LENGTH: Length
 
-  datatype Buffer<T> =
+  datatype Buffer<T(==)> =
     | Node(payload: T, next: Buffer)
     | Tail
     {
@@ -13,11 +13,27 @@ module NoC {
         case Tail => 0
       }
 
-      function append(p: T): Buffer<T> {
+      function append(p: T): Buffer<T>
+        ensures this.is_prefix_of(append(p))
+        ensures append(p).length() == this.length() + 1
+      {
         match this
         case Node(payload, next) => Node(payload, next.append(p))
         case Tail => Node(p, Tail)
       }
+
+      predicate is_prefix_of(b: Buffer<T>) {
+        match (this, b)
+        case (Tail, Tail) => true
+        case (Node(_, _), Tail) => false
+        case (Tail, Node(_, _)) => true
+        case (Node(p, n), Node(p', n')) => p == p' && n.is_prefix_of(n')
+      }
+
+      static lemma EqualIsPrefix(a: Buffer<T>, b: Buffer<T>)
+        requires a == b
+        ensures a.is_prefix_of(b) && b.is_prefix_of(a)
+      {}
     }
 
   datatype Direction =
@@ -27,12 +43,15 @@ module NoC {
     | West
     | Local
 
-  class Router<T> {
-    var North: Buffer<T>
-    var East:  Buffer<T>
-    var South: Buffer<T>
-    var West:  Buffer<T>
-    var Local: Buffer<T>
+  method DiscreteRandom(low: nat, high: nat) returns (r: nat)
+    ensures {:axiom} low <= r <= high
+
+  class Router {
+    var North: Buffer<nat>
+    var East:  Buffer<nat>
+    var South: Buffer<nat>
+    var West:  Buffer<nat>
+    var Local: Buffer<nat>
 
     constructor()
       ensures North.length() == 0 && East.length() == 0 && South.length() == 0 && West.length() == 0 && Local.length() == 0
@@ -44,38 +63,44 @@ module NoC {
       Local := Tail;
     }
 
-    method insertLocal(payload: T)
-      modifies this.Local 
+    method generateFlits(cycle: nat, dim: nat, id: nat)
+      requires 2 <= dim
+      requires 0 <= id < dim*dim
+      requires this.Local.length() <= BUFFER_LENGTH
+      modifies this
+      ensures old(this.Local).is_prefix_of(this.Local)
+      ensures this.Local.length() <= BUFFER_LENGTH
     {
-      this.Local := this.Local.append(payload);
+      if cycle % 3 >= 3 {
+        return;
+      }
+
+      if this.Local.length() < BUFFER_LENGTH {
+        var dest_id := DiscreteRandom(0, dim*dim - 2);
+        if dest_id >= id {
+          dest_id := dest_id + 1;
+        }
+        assert dest_id != id;
+        this.Local := this.Local.append(dest_id);
+      } else {
+        assert old(this.Local) == this.Local;
+        Buffer.EqualIsPrefix(old(this.Local), this.Local);
+      }
     }
   }
 
-  type NoC = n: seq<seq<Router<nat>>> | |n| >= 2 && (forall y :: 0 <= y < |n| ==> |n[y]| == |n|) witness *
+  class NoC {
+    const dim: nat
+    var routers: seq<seq<Router>>
 
-  method generateFlits(n: NoC, cycle: nat) returns (n': NoC)
-  {
-    n' := n;
-
-    if cycle % 3 >= 3 {
-      return;
-    }
-
-    var dim := |n|;
-    var y := 0;
-
-    while y < dim
+    constructor(dim: nat)
+      ensures dim == this.dim
+      ensures |routers| == this.dim
+      ensures forall y :: 0 <= y < this.dim ==> |routers[y]| == this.dim
     {
-      var x := 0;
-      while x < dim
-      {
-        if n'[y][x].Local.length() < BUFFER_LENGTH {
-          var dest_id :| 0 <= dest_id < dim * dim && dest_id != y*dim + x;
-          n'[y][x].Local := n'[y][x].Local.append(dest_id);
-        }
-        x := x + 1;
-      }
-      y := y + 1;
+      this.dim := dim;
+      new;
+      routers := seq(this.dim, y => seq(x, _ => new Router()));
     }
   }
 }
